@prefix owl:    <http://www.w3.org/2002/07/owl#> .
@prefix dc:     <http://purl.org/dc/elements/1.1/> .
@prefix rdf:    <http://www.w3.org/1999/02/22-rdf-syntax-ns#> .
@prefix rdfs:   <http://www.w3.org/2000/01/rdf-schema#> .
@prefix xsd:    <http://www.w3.org/2000/10/XMLSchema#> .
@prefix psg:    <http://fr.gdd.passage/engine-vocabulary#> .
@prefix ja:     <http://jena.hpl.hp.com/2005/11/Assembler#> .
@prefix fuseki:  <http://jena.apache.org/fuseki#> .

## This vocabulary aims to define the configuration of an available engine
## which are either PASSAGE, or RAW.
## In addition, we would like to be able to create custom ones, by
## defining the class to instantiate for each operator of SPARQL

## To produce this document, we took an example of HeFQUIN available at:
## <https://github.com/LiUSemWeb/HeFQUIN/blob/main/hefquin-vocabs/engineconf.ttl>

<http://fr.gdd.passage/engine-vocabulary> rdf:type owl:Ontology ;
    dc:creator       "Chat-Wane" ;
    dc:date          "2025-24-02" ;
    dc:format        "RDF" ;
    # TODO dc:identifier w3id.org
    dc:title         "Vocabulary for describing engines in PASSAGE"@en ;
    rdfs:label       "Vocabulary for describing engines in PASSAGE"@en .

## Operations

psg:query_w_args rdf:type fuseki:Operation ;
    rdfs:label       "SPARQL query with args"@en ;
    rdfs:comment     "SPARQL query operation for Fuseki that allows reading body's and header's arguments."@en ;
    fuseki:implementation "fr.gdd.passage.cli.operations.SPARQL_QueryDatasetWithHeaders" ;
    fuseki:name      "query_w_args" .

## Engines

psg:SPARQLEngine rdf:type owl:Class ;
    rdfs:label       "SPARQL engine configuration"@en ;
    rdfs:comment     "Abstract class of SPARQL engine configuration."@en .

psg:PassageEngine rdf:type owl:Class ;
    rdfs:subClassOf  psg:SPARQLEngine ;
    rdfs:label       "PASSAGE configuration"@en ;
    rdfs:comment     "Class of configuration for the PASSAGE engine."@en .

psg:RawEngine rdf:type owl:Class ;
    rdfs:subClassOf  psg:SPARQLEngine ;
    rdfs:label       "RAW configuration"@en ;
    rdfs:comment     "Class of configuration for the RAW engine."@en .

psg:CustomEngine rdf:type owl:Class ;
    rdfs:subClassOf  psg:SPARQLEngine ;
    rdfs:label       "Custom configuration"@en ;
    rdfs:comment     "Class of configuration to define its own custom SPARQL engine operator per operator."@en .

psg:engine rdf:type rdf:Property ;
    rdfs:range       psg:SPARQLEngine ;
    # TODO rdfs:domain
    rdfs:label       "SPARQL query engine"@en ;
    rdfs:comment     "Specifies the SPARQL query engines to use with the service."@en .


## Datasets

psg:DatasetBlazegraph rdf:type owl:Class ;
    rdfs:subClassOf  ja:dataset ;
    rdfs:label       "Blazegraph dataset"@en ;
    rdfs:comment     "An instance of this class defines a dataset with a Blazegraph backend."@en .

psg:DatasetHDT rdf:type owl:Class ;
    rdfs:subClassOf  ja:dataset ;
    rdfs:label       "HDT dataset"@en ;
    rdf:comment      "An instance of this class defines a dataset with an HDT backend."@en .


## Properties

psg:location rdf:type rdf:Property;
    rdfs:label       "Dataset location"@en ;
    rdfs:comment     "The location of the file to read to create the dataset."@en .

psg:timeout rdf:type rdf:Property;
    rdfs:label       "Query execution timeout"@en ;
    rdfs:comment     "Timeout on SPARQL query execution. Depending on the query engine, a specific behavior is associated."@en .

psg:max_results rdf:type rdf:Property;
    rdfs:label       "Maximum number of results"@en ;
    rdfs:comment     "Maximum number of results returned by a query execution."@en .

psg:parallel rdf:type rdf:Property;
    rdfs:label       "Maximum number of threads"@en ;
    rdfs:comment     "Maximum number of threads allocated to each SPARQL query execution."@en .

psg:force_order rdf:type rdf:Property ;
    rdfs:label       "Force order of triple/quad patterns"@en ;
    rdfs:comment     "Defines if the engine should try to optimize the join order or not."@en .

## TODO describe supported operators

## TODO Custom engines
